fixed compiler errors

verify.dfy
@@ -1,25 +1,30 @@
-var maxSize := 20;
-
 class Socket 
 {
+  var maxSize : int;
+
   var keySize : int;
   var privateKey : string;
   var remHostname : string;
   var alpnProtos : array<string>;
-  var cipherSuites : array<SSL_CIPHER>; //fix this
+  var cipherSuites : array<string>; // FIXME - should be array of type SSL_CIPHER
 
   method Init(kSize : int, pKey : string, rHostname : string)
   modifies this;
+  ensures fresh(alpnProtos);
+  ensures fresh(cipherSuites);
   {
+    maxSize := 20;
+
     keySize := kSize;
-    privateKay := pKey;
+    privateKey := pKey;
     remHostname := rHostname;
     alpnProtos := new string[maxSize];
     cipherSuites := new string[maxSize];
   }
   
-  method isSecure()
+  predicate isSecure()
   {
+    true
   }
 }
 
